Replace evaluation rule for fix to not use explicit substitution

src/SmallStep.v
@@ -13,27 +13,6 @@ Module SmallStep (P : PAT).
   Module SmallStep1 (M : MATCH).
     Export M.
 
-    Inductive is_value : term -> Prop :=
-    | VLam   : forall ty t,
-        is_value (TmLam ty t)
-    | VTyLam : forall k t,
-        is_value (TmTyLam k t)
-    | VProd : forall v1 v2,
-        is_value v1 ->
-        is_value v2 ->
-        is_value (TmProd v1 v2)
-    | VCon : forall K ty v,
-        is_value v ->
-        is_value (TmCon K ty v)
-    | VSem : forall ty p t,
-        is_value (TmSem ty p t)
-    | VComp : forall v1 v2,
-        is_value v1 ->
-        is_value v2 ->
-        is_value (TmComp v1 v2).
-    #[export]
-     Hint Constructors is_value : mcore.
-
     Fixpoint push_value (f : term -> term) (t : term) : term :=
       match t with
       | TmLam ty t' => TmLam ty (f t')
@@ -87,8 +66,12 @@ Module SmallStep (P : PAT).
         TmApp (TmLam ty t) v --> [0 ~> v]t
     | ETyApp : forall k t ty,
         TmTyApp (TmTyLam k t) ty --> [{0 ~> ty}]t
-    | EFix : forall ty t,
-        TmFix (TmLam ty t) --> [0 ~> TmFix (TmLam ty t)]t
+    | EFix : forall ty1 ty2 t,
+        TmFix (TmLam (TyArr ty1 ty2) t) -->
+              TmApp
+              (TmLam (TyArr ty1 ty2) t)
+              (TmLam ty1
+                     (TmApp (TmFix (TmLam (TyArr ty1 ty2) t)) (TmBVar 0)))
     | EProj1 : forall v1 v2,
         is_value v1 ->
         is_value v2 ->
