src/Soundness.v
@@ -34,14 +34,17 @@ Module Soundness (P : PAT).
           rewrite (tsubst_intro X)...
           rewrite (tsubst_t_intro X)...
           apply_empty* ok_term_tsubst. }
-        { Case "TmFix". inverts hasType.
-          pick_fresh x. rewrite~ (subst_intro x).
-          apply_empty* ok_term_subst. }
+        { Case "TmFix". inverts hasType. inverts H3.
+          constructors*. apply_fresh* TLam.
+          replace ([0 ~> TmFVar y] TmApp (TmFix (TmLam (TyArr ty1 ty2) t0)) (TmBVar 0))
+            with (TmApp ([0 ~> TmFVar y] TmFix (TmLam (TyArr ty1 ty2) t0)) (TmFVar y))
+            by solve_var.
+          rewrite* open_lc. constructors*. apply_empty* ok_term_weakening. }
         { Case "TmProj1". inverts* hasType. }
         { Case "TmProj2". inverts* hasType. }
         { Case "TmMatchThen". pick_fresh M. pick_fresh x. rewrite~ (subst_intro x).
           assert (Gamma & M ~ BindMatch t p true |= [x => v'] ([0 ~> TmFVar x] t1) ~: ty2).
-          { apply_empty~ ok_term_subst ; try constructors*. apply* match1_ok_pat.
+          { apply_empty~ ok_term_subst ; try constructors*. applys* match1_value H10. apply* match1_ok_pat.
             apply_empty~ ok_pat_weakening ; try constructors*. apply H. }
           replaces true with (is_some (match1 t p)) in H4. rewrite~ H10.
           apply_empty ok_term_drop_match... }
@@ -61,7 +64,7 @@ Module Soundness (P : PAT).
           assert (i < length ps0) by apply* matchN_length.
           forwards* (L&ty1'&Hpat&Htype) : ok_term_get_cases_inv i.
           remember (nth i bs) ; pick_fresh x ; substs. rewrite~ (subst_intro x).
-          apply_empty* ok_term_subst. apply* matchN_ok_pat. }
+          apply_empty* ok_term_subst. applys* matchN_value H6. apply* matchN_ok_pat. }
       Qed.
 
       Definition no_vars (Gamma : env) : Prop :=
